typing sessions (some conditions like guardedness is missing)

types/typecheck.v
@@ -1,4 +1,4 @@
-Require Import ST.processes.process ST.types.local ST.subtyping.subtyping ST.src.st ST.negations.nsubtyping.
+Require Import ST.processes.process ST.types.local ST.subtyping.subtyping ST.src.st ST.negations.nsubtyping ST.types.typenv.
 From mathcomp Require Import all_ssreflect.
 From Paco Require Import paco.
 Require Import ST.src.stream.
@@ -148,7 +148,6 @@ Inductive typ_expr: ctxS -> expr -> local.sort -> Prop :=
                              typ_expr c (e_plus e1 e2) sint
   | sc_det  : forall c e1 e2 s, typ_expr c e1 s -> typ_expr c e2 s -> typ_expr c (e_det e1 e2) s.
 
-
 (* Inductive tcE: theta -> expr -> local.sort -> Prop :=
   | tce_iv1: forall c n, tcE c (isval (vint n)) sint
   | tce_iv2: forall c n, tcE c (isval (vbool n)) sbool
@@ -158,13 +157,31 @@ Inductive typ_expr: ctxS -> expr -> local.sort -> Prop :=
   | tce_igt: forall c a s, Some s = tcAE c a -> tcE c (isgt a) sbool
   | tce_iss: forall c e s' s, is_ss s s' = true -> tcE c e s' -> tcE c e s. *)
 
+Inductive typ_queue: mqueue -> queue -> Prop :=
+  | tq_nil : typ_queue nil nil
+  | tq_cons: forall p l v s xs ys cs, typ_expr cs v s -> typ_queue xs ys -> typ_queue ((p,l,v)::xs) ((p,l,s)::ys).
+
+Lemma typ_queu_app: forall q1 m1 q2 m2, typ_queue q1 m1 -> typ_queue q2 m2 -> typ_queue (q1 ++ q2) (m1 ++ m2).
+Proof. intro q1.
+       induction q1; intros.
+       - inversion H. subst. simpl. easy.
+       - case_eq m1; intros.
+         + subst. inversion H.
+         + subst.
+           destruct a as ((r1,l1),s1).
+           destruct p as ((r2,l2),s2).
+           simpl.
+           inversion H. subst.
+           apply tq_cons with (cs := cs). easy.
+           apply IHq1; easy.
+Qed.
 
 Inductive typ_proc: ctxS -> ctxT -> process -> local -> Prop :=
   | tc_inact: forall cs ct,     typ_proc cs ct (ps_end) (lt_end)
   | tc_var  : forall cs ct s t, nth s ct None = Some t -> (* wfC t -> *)
                                 typ_proc cs ct (ps_var s) t
-  | tc_mu   : forall cs ct p t,       typ_proc cs (Some t :: ct) p t ->
-                                      typ_proc cs ct (ps_mu p) t
+  | tc_mu   : forall cs ct p t, typ_proc cs (Some t :: ct) p t ->
+                                typ_proc cs ct (ps_mu p) t
   | tc_ite  : forall cs ct e p1 p2 T, typ_expr cs e sbool ->
                                       typ_proc cs ct p1 T ->
                                       typ_proc cs ct p2 T ->
@@ -178,6 +195,15 @@ Inductive typ_proc: ctxS -> ctxT -> process -> local -> Prop :=
   | tc_snd  : forall cs ct p l e P S T, typ_expr cs e S ->
                                         typ_proc cs ct P T ->
                                         typ_proc cs ct (ps_send p l e P) (lt_send p (cons (l, S, T) nil)).
+
+Inductive ForallT (P : participant -> process -> mqueue -> Prop) : session -> Prop := 
+  | ForallT_mono: forall pt op h, P pt op h -> ForallT P (pt <-- op | h)
+  | ForallT_par : forall (M1 M2 : session), ForallT P M1 -> ForallT P M2 -> ForallT P (M1 |||| M2). 
+
+(*add guardedness of local types and processes + make sure that the typing context and the session having exact same participants with no duplications*)
+Inductive typ_sess : session -> ctx -> Prop := 
+  | t_sess : forall M G, ForallT (fun u P h => exists gamma T, M.find u G = Some (gamma, T) /\ typ_queue h gamma /\ typ_proc nil nil P T) M ->
+                         typ_sess M G.
 
 Lemma remark4_5: forall cs ct e, typ_expr cs e sbool ->
                                  typ_proc cs ct (ps_ite e (ps_send "q" "l1" (e_val (vint 1%Z)) (ps_send "r" "l2" (e_val (vint 2)) ps_end)) 
