examples/Example2_3.v
@@ -10,28 +10,28 @@ Require Import Morphisms.
 Local Open Scope string_scope.
 
 Definition M1 (p q: participant) (l: label): session :=
-  (p <-- ps_receive q [(l,ps_end)] | nilq) |||| (q <-- ps_send p l (e_val (vint 42%Z)) ps_end | nilq).
+  (p <-- ps_receive q [(l,ps_end)] | nil) |||| (q <-- ps_send p l (e_val (vint 42%Z)) ps_end | nil).
 
 Definition M1' (p q: participant) (l: label): session :=
-  (p <-- ps_end | nilq) |||| (q <-- ps_end | nilq).
+  (p <-- ps_end | nil) |||| (q <-- ps_end | nil).
 
 Example redM1: forall (p q: participant) (l: label), beta_multistep (M1 p q l) (M1' p q l).
 Proof. intros.
        unfold beta_multistep, M1, M1'.
        setoid_rewrite scomm.
        apply multi_step with (y := 
-         ((q <-- ps_end | (conq nilq (mesq p l (e_val (vint 42)) nilq))) ||||
-          (p <-- ps_receive q [(l,ps_end)] | nilq))).
-       apply r_send. simpl.
-       constructor.
+         ((q <-- ps_end | (nil ++ [(p,l,(e_val (vint 42)))])) ||||
+          (p <-- ps_receive q [(l,ps_end)] | nil))).
+       apply r_send.
+       constructor. simpl.
 
        setoid_rewrite scomm.
        apply multi_step with (y := 
-         (((p <-- subst_expr_proc (ps_receive q [(l, ps_end)]) (e_val (vint 42)) l 0 0 | nilq) |||| 
-          (q <-- ps_end | nilq)))).
+         (((p <-- subst_expr_proc (ps_receive q [(l, ps_end)]) (e_val (vint 42)) l 0 0 | nil) |||| 
+          (q <-- ps_end | nil)))).
        specialize (r_rcv p q l ([(l, ps_end)])
-                         (vint 42) (ps_end) nilq nilq
-                         (p <-- ps_end | nilq)
+                         (vint 42) (ps_end) nil nil
+                         (p <-- ps_end | nil)
        ); intro HR.
        setoid_rewrite scomm in HR.
        setoid_rewrite sann in HR.
@@ -53,18 +53,18 @@ Definition PBob: process :=
 Definition PCarol: process :=
   ps_receive "Bob" [("l2", ps_send "Alice" "l3" (e_succ (e_var 1))  ps_end)].
 
-Definition MS: session := ("Alice" <-- PAlice | nilq) |||| ("Bob" <-- PBob | nilq) |||| ("Carol" <-- PCarol | nilq).
+Definition MS: session := ("Alice" <-- PAlice | nil) |||| ("Bob" <-- PBob | nil) |||| ("Carol" <-- PCarol | nil).
 
-Definition MS': session := ("Alice" <-- ps_end | nilq) |||| ("Bob" <-- ps_end | nilq) |||| ("Carol" <-- ps_end | nilq).
+Definition MS': session := ("Alice" <-- ps_end | nil) |||| ("Bob" <-- ps_end | nil) |||| ("Carol" <-- ps_end | nil).
 
 Example redMS: beta_multistep MS MS'.
 Proof. intros.
        unfold beta_multistep, MS, MS', PAlice.
        apply multi_step with
-       (y := (("Alice" <-- (ps_receive "Carol" [("l3", ps_end)]) | conq nilq (mesq "Bob" "l1" (e_val (vnat 50)) nilq)) ||||
-             ("Bob" <-- PBob | nilq)) |||| ("Carol" <-- PCarol | nilq)).
+       (y := (("Alice" <-- (ps_receive "Carol" [("l3", ps_end)]) | (nil ++ [("Bob","l1",(e_val (vnat 50)))])) ||||
+             ("Bob" <-- PBob | nil)) |||| ("Carol" <-- PCarol | nil)).
        setoid_rewrite sassoc.
-       apply r_send. simpl.
+       apply r_send.
        constructor.
 
        setoid_rewrite sassoc.
@@ -73,9 +73,9 @@ Proof. intros.
        setoid_rewrite <- sassoc.
 
        apply multi_step with
-       (y := ("Bob" <-- subst_expr_proc (PBob) (e_val (vnat 50)) "l1"  0 0 | nilq)
-              |||| ("Alice" <-- ps_receive "Carol" [("l3", ps_end)] | nilq)
-              |||| ("Carol" <-- PCarol | nilq)).
+       (y := ("Bob" <-- subst_expr_proc (PBob) (e_val (vnat 50)) "l1"  0 0 | nil)
+              |||| ("Alice" <-- ps_receive "Carol" [("l3", ps_end)] | nil)
+              |||| ("Carol" <-- PCarol | nil)).
        apply r_rcv.
        simpl. 
        unfold PCarol.
@@ -84,11 +84,11 @@ Proof. intros.
        setoid_rewrite <- sassoc.
 
        apply multi_step with
-       (y := ((("Bob" <-- ps_end | conq nilq (mesq "Carol" "l2" (e_val (vnat 100)) nilq) )
-               |||| ("Carol" <-- ps_receive "Bob" [("l2", ps_send "Alice" "l3" (e_succ (e_var 1)) ps_end)] | nilq))
-               |||| ("Alice" <-- ps_receive "Carol" [("l3", ps_end)] | nilq))).
+       (y := ((("Bob" <-- ps_end | (nil ++ [("Carol","l2",(e_val (vnat 100)))]) )
+               |||| ("Carol" <-- ps_receive "Bob" [("l2", ps_send "Alice" "l3" (e_succ (e_var 1)) ps_end)] | nil))
+               |||| ("Alice" <-- ps_receive "Carol" [("l3", ps_end)] | nil))).
        setoid_rewrite sassoc.
-       apply r_send. simpl.
+       apply r_send.
        constructor.
 
        setoid_rewrite sassoc.
@@ -97,9 +97,9 @@ Proof. intros.
        setoid_rewrite <- sassoc.
 
        apply multi_step with
-       (y := ((("Carol" <-- subst_expr_proc (ps_receive "Bob" [("l2", ps_send "Alice" "l3" (e_succ (e_var 1)) ps_end)]) (e_val (vnat 100)) "l2" 0 0 | nilq)
-                 |||| ("Bob" <-- ps_end | nilq))
-                 |||| ("Alice" <-- ps_receive "Carol" [("l3", ps_end)] | nilq))).
+       (y := ((("Carol" <-- subst_expr_proc (ps_receive "Bob" [("l2", ps_send "Alice" "l3" (e_succ (e_var 1)) ps_end)]) (e_val (vnat 100)) "l2" 0 0 | nil)
+                 |||| ("Bob" <-- ps_end | nil))
+                 |||| ("Alice" <-- ps_receive "Carol" [("l3", ps_end)] | nil))).
        apply r_rcv. simpl.
        simpl.
 
@@ -107,9 +107,9 @@ Proof. intros.
        setoid_rewrite <- sassoc.
 
        apply multi_step with
-       (y := ((("Carol" <-- ps_end | conq nilq (mesq "Alice" "l3" (e_val (vnat 101)) nilq) )
-               |||| ("Alice" <-- ps_receive "Carol" [("l3", ps_end)] | nilq))
-               |||| ("Bob" <-- ps_end | nilq))).
+       (y := ((("Carol" <-- ps_end | (nil ++ [("Alice","l3",(e_val (vnat 101)))]))
+               |||| ("Alice" <-- ps_receive "Carol" [("l3", ps_end)] | nil))
+               |||| ("Bob" <-- ps_end | nil))).
        setoid_rewrite sassoc.
        apply r_send. simpl.
        specialize (ec_succ (e_val (vnat 100)) 100); intro He. apply He. constructor.
@@ -120,9 +120,9 @@ Proof. intros.
        setoid_rewrite <- sassoc.
 
       apply multi_step with
-      (y := ((("Alice" <-- subst_expr_proc (ps_receive "Carol" [("l3", ps_end)]) (e_val (vnat 101)) "l3" 0 0 | nilq) 
-             |||| ("Carol" <-- ps_end | nilq))
-             |||| ("Bob" <-- ps_end | nilq))).
+      (y := ((("Alice" <-- subst_expr_proc (ps_receive "Carol" [("l3", ps_end)]) (e_val (vnat 101)) "l3" 0 0 | nil) 
+             |||| ("Carol" <-- ps_end | nil))
+             |||| ("Bob" <-- ps_end | nil))).
       apply r_rcv. simpl.
 
       apply multi_refl.
